<?xml version="1.0"?>
<rdf:RDF xmlns="http://www.iri.upc.edu/groups/perception/OCRA/ont/ocra_cloth.owl#"
     xml:base="http://www.iri.upc.edu/groups/perception/OCRA/ont/ocra_cloth.owl"
     xmlns:dc="http://purl.org/dc/elements/1.1/"
     xmlns:DUL="http://www.ontologydesignpatterns.org/ont/dul/DUL.owl#"
     xmlns:owl="http://www.w3.org/2002/07/owl#"
     xmlns:rdf="http://www.w3.org/1999/02/22-rdf-syntax-ns#"
     xmlns:xml="http://www.w3.org/XML/1998/namespace"
     xmlns:xsd="http://www.w3.org/2001/XMLSchema#"
     xmlns:ocra="http://www.iri.upc.edu/groups/perception/OCRA/ont/ocra.owl#"
     xmlns:rdfs="http://www.w3.org/2000/01/rdf-schema#">
    <owl:Ontology rdf:about="http://www.iri.upc.edu/groups/perception/OCRA/ont/ocra_home.owl">
        <owl:imports rdf:resource="http://www.iri.upc.edu/groups/perception/OCRA/ont/ocra.owl"/>
    </owl:Ontology>
    


    <!-- 
    ///////////////////////////////////////////////////////////////////////////////////////
    //
    // Object Properties
    //
    ///////////////////////////////////////////////////////////////////////////////////////
     -->

    


    <!-- http://www.iri.upc.edu/groups/perception/OCRA/ont/ocra_home.owl#hasFlavor -->

    <owl:ObjectProperty rdf:about="http://www.iri.upc.edu/groups/perception/OCRA/ont/ocra_home.owl#hasFlavor">
        <rdfs:subPropertyOf rdf:resource="http://www.ontologydesignpatterns.org/ont/dul/DUL.owl#hasQuality"/>
        <rdfs:comment xml:lang="en">Relationship between Drinks and their flavor(s). 

Note that a drink can have several flavors. Furthermore, this relation can be generalized to hold between other entities and their flavor (e.g., food, dishes, etc.). However, for this application ontology it has been decided to model it only for the objects of interest: drinks.</rdfs:comment>
        <rdfs:label>has flavor</rdfs:label>
    </owl:ObjectProperty>
    


    <!-- http://www.iri.upc.edu/groups/perception/OCRA/ont/ocra_home.owl#hasTemperature -->

    <owl:ObjectProperty rdf:about="http://www.iri.upc.edu/groups/perception/OCRA/ont/ocra_home.owl#hasTemperature">
        <rdfs:subPropertyOf rdf:resource="http://www.ontologydesignpatterns.org/ont/dul/DUL.owl#hasQuality"/>
        <rdfs:comment xml:lang="en">Relationship between Drinks and their Temperature.

Note that this relation can be generalized to hold between other entities and their temperature (e.g., the volume of a room, a car, a city, etc.). However, for this application ontology it has been decided to model it only for the objects of interest: drinks.</rdfs:comment>
        <rdfs:label>has temperature</rdfs:label>
    </owl:ObjectProperty>
    


    <!-- 
    ///////////////////////////////////////////////////////////////////////////////////////
    //
    // Classes
    //
    ///////////////////////////////////////////////////////////////////////////////////////
     -->

    


    <!-- http://www.iri.upc.edu/groups/perception/OCRA/ont/ocra_home.owl#Drink -->

    <owl:Class rdf:about="http://www.iri.upc.edu/groups/perception/OCRA/ont/ocra_home.owl#Drink">
        <rdfs:subClassOf rdf:resource="http://www.ontologydesignpatterns.org/ont/dul/DUL.owl#Object"/>
        <rdfs:comment xml:lang="en">An Ojbect that refers to a general conceptualization of (an amount of) liquid that is (or can be) taken into the body through the mouth. 

This class can be used to represent both a physical object (e.g. a cup of tea), and a social object referring to the physical one (e.g. would you like to have a tea?).</rdfs:comment>
        <rdfs:label xml:lang="en">Drink</rdfs:label>
    </owl:Class>
    

</rdf:RDF>



<!-- Generated by the OWL API (version 4.5.6.2018-09-06T00:27:41Z) https://github.com/owlcs/owlapi -->

